Pushed normalization-related changes through so that progs now builds; semax_prog statements and (old) Espec constructions at the end of verifXXX.v files now need to be stated wrt (normalizeFunspecs Gprog) rather than Gprog

floyd/SeparationLogicAsLogic.v
@@ -297,7 +297,7 @@ forall nNEP,
   @semax_func Espec V G C ge ((id, Internal f)::fs)
        ((id, mk_funspec (params, retsig) cc A nP Q nNEP NEQ)::G')
 
-| semax_func_cons_ext: forall {Espec: OracleKind}
+| semax_func_cons_ext_with_normalization: forall {Espec: OracleKind}
       (V: varspecs) (G: funspecs) {C: compspecs} ge fs id ef (argtypes:typelist) retsig A P Q (*NEP NEQ*)
       (params:list (ident * type))
       (G': funspecs) cc (ids: list ident) b,
@@ -330,13 +330,15 @@ forall nNEP,
   semax_func V G ge ((id, External ef argtypes retsig cc)::fs)
        ((id, mk_funspec (params, retsig) cc A nP Q 
                  (*(rename_pre_super_non_expansive NEP nids ids)*)NEP NEQ)  :: G')
-(*WAS:
+
+| semax_func_cons_ext:
   forall {Espec: OracleKind},
    forall (V: varspecs) (G: funspecs) {C: compspecs} ge fs id ef argsig retsig A P Q NEP NEQ
           argsig'
           (G': funspecs) cc (ids: list ident) b,
       ids = map fst argsig' -> (* redundant but useful for the client,
                to calculate ids by reflexivity *)
+(*New*)  funspec_normalized (mk_funspec (argsig', retsig) cc A P Q NEP NEQ) = true -> 
       argsig' = zip_with_tl ids argsig ->
       ef_sig ef =
       mksignature
@@ -349,11 +351,12 @@ forall nNEP,
          (Q ts x (make_ext_rval gx ret)
             && !!step_lemmas.has_opttyp ret (opttyp_of_type retsig)
             |-- !!tc_option_val retsig ret)) ->
-(*new*) Genv.find_symbol ge id = Some b -> Genv.find_funct_ptr ge b = Some (External ef argsig retsig cc) ->
+      Genv.find_symbol ge id = Some b -> Genv.find_funct_ptr ge b = Some (External ef argsig retsig cc) ->
       @semax_external Espec ids ef A P Q ->
       semax_func V G ge fs G' ->
       semax_func V G ge ((id, External ef argsig retsig cc)::fs)
-           ((id, mk_funspec (argsig', retsig) cc A P Q NEP NEQ)  :: G')*)
+           ((id, mk_funspec (argsig', retsig) cc A P Q NEP NEQ)  :: G')
+
 | semax_func_mono: forall  {Espec CS CS'} (CSUB: cspecs_sub CS CS') ge ge'
   (Gfs: forall i,  sub_option (Genv.find_symbol ge i) (Genv.find_symbol ge' i))
   (Gffp: forall b, sub_option (Genv.find_funct_ptr ge b) (Genv.find_funct_ptr ge' b))
@@ -1230,8 +1233,9 @@ Definition semax_func_nil := @AuxDefs.semax_func_nil (@Def.semax_external).
 
 Definition semax_func_cons := @AuxDefs.semax_func_cons (@Def.semax_external).
 
+Definition semax_func_cons_ext_with_normalization := @AuxDefs.semax_func_cons_ext_with_normalization (@Def.semax_external).
 Definition semax_func_cons_ext := @AuxDefs.semax_func_cons_ext (@Def.semax_external).
-  
+
 Theorem semax_ifthenelse :
   forall {CS: compspecs} {Espec: OracleKind},
    forall Delta P (b: expr) c d R,
