progs/verif_logical_compare.v
@@ -142,7 +142,7 @@ Qed.
 Existing Instance NullExtension.Espec.
 
 Lemma prog_correct:
-  semax_prog prog tt Vprog Gprog.
+  semax_prog prog tt Vprog (normalizeFunspecs Gprog).
 Proof.
 prove_semax_prog.
 semax_func_cons body_do_or.
