progs/verif_sumarray.v
@@ -120,7 +120,7 @@ Qed.
 Existing Instance NullExtension.Espec.
 
 Lemma prog_correct:
-  semax_prog prog tt Vprog Gprog.
+  semax_prog prog tt Vprog (normalizeFunspecs Gprog).
 Proof.
   prove_semax_prog.
   semax_func_cons body_sumarray.
